Extract destruct lemmas for IOStar to a separate file

seiostar/IOStar.fst
@@ -141,29 +141,6 @@ let lem_thetaP_bind #a #b (m:io a) (k:a -> io b) :
          dump "H")
 **)
 
-#push-options "--split_queries always"
-val lem_theta_call (o:io_ops) (args:io_args o) (res:io_res o args) (h:history) :
-  Lemma (requires io_post h o args res)
-        (ensures thetaP (io_call o args) h [op_to_ev o args res] res)
-let lem_theta_call o args res h =
-  introduce forall (p:hist_post h (io_res o args)). (theta (io_call o args)) h p ==> p [op_to_ev o args res] res with begin
-    introduce (theta (io_call o args)) h p ==> p [op_to_ev o args res] res with _. begin
-      assert ((hist_bind (op_wp o args) (fun (r:io_res o args) -> theta (Return r))) h p ==>
-              (hist_bind (to_hist (fun h_ -> io_pre h_ o args) (fun h_ res_ lt_ -> io_post h_ o args res_ /\ lt_ == [op_to_ev o args res_])) (fun (r:io_res o args) -> theta (Return r))) h p) by (compute ());
-      eliminate forall (lt':local_trace h) (r':io_res o args). lt' == [op_to_ev o args r'] ==>
-        (theta (Return r')) (h++lt') (fun (lt'':local_trace (h++lt')) (r'':io_res o args) -> p (lt' @ lt'') r'')
-        with [op_to_ev o args res] res
-    end
-  end
-#pop-options
-
-val destruct_thetaP_call (o:io_ops) (args:io_args o) (h:history) (lt:local_trace h) (fs_r:io_res o args) :
-  Lemma (requires thetaP (io_call o args) h lt fs_r)
-        (ensures lt == [op_to_ev o args fs_r] /\ io_post h o args fs_r)
-let destruct_thetaP_call o args h lt fs_r =
-  let p : hist_post h (io_res o args) = fun lt' r' -> lt' == [op_to_ev o args r'] /\ io_post h o args r' in
-  assert (theta (io_call o args) h p) by (compute ());
-  assert (p lt fs_r)
 
 let lem_thetaP_return #a (x:a) (h:history) :
   Lemma (thetaP (return x) h [] x) =
@@ -187,112 +164,18 @@ let lem_thetaP_bind #a #b (m:io a) (h:history) (lt1:local_trace h) (fs_r_m:a) (k
   end
 #pop-options
 
-let thetaP_shift_op_lt #t (o:io_ops) (args:io_args o) (k:io_res o args -> io t) (r:io_res o args) (h:history) (lt:local_trace h)
-  : Lemma
-      (requires (lt == [op_to_ev o args r]))
-      (ensures (forall (lt':local_trace (h++lt)) fs_r . thetaP (k r) (h ++ lt) lt' fs_r ==> thetaP (Call o args k) h (lt@lt') fs_r))
-  =
-  introduce forall (lt':local_trace (h++lt)) fs_r . thetaP (k r) (h ++ lt) lt' fs_r ==> thetaP (Call o args k) h (lt@lt') fs_r with begin
-    introduce thetaP (k r) (h ++ lt) lt' fs_r ==> thetaP (Call o args k) h (lt@lt') fs_r with _. begin
-      introduce forall (p:hist_post h t). theta (Call o args k) h p ==> p (lt@lt') fs_r with begin
-        introduce theta (Call o args k) h p ==> p (lt@lt') fs_r with _. begin
-          assert (hist_bind (op_wp o args) (fun r -> theta (k r)) h p);
-          assert (forall (lt:local_trace h) (r:io_res o args). lt == [op_to_ev o args r] ==> theta (k r) (h++lt) (hist_post_shift h p lt)) by (
-            binder_retype (nth_binder (-1));
-              norm [delta_only [`%hist_bind;`%op_wp;`%to_hist;`%io_post;`%io_pre;`%hist_post_bind'];iota];
-            trefl ());
-          eliminate forall (lt:local_trace h) (r:io_res o args). lt == [op_to_ev o args r] ==> theta (k r) (h++lt) (hist_post_shift h p lt)
-            with lt r;
-          eliminate forall (p':hist_post (h++lt) t). theta (k r) (h++lt) p' ==> p' lt' fs_r
-            with (hist_post_shift h p lt)
-        end
-      end
+#push-options "--split_queries always"
+val lem_thetaP_call (o:io_ops) (args:io_args o) (res:io_res o args) (h:history) :
+  Lemma (requires io_post h o args res)
+        (ensures thetaP (io_call o args) h [op_to_ev o args res] res)
+let lem_thetaP_call o args res h =
+  introduce forall (p:hist_post h (io_res o args)). (theta (io_call o args)) h p ==> p [op_to_ev o args res] res with begin
+    introduce (theta (io_call o args)) h p ==> p [op_to_ev o args res] res with _. begin
+      assert ((hist_bind (op_wp o args) (fun (r:io_res o args) -> theta (Return r))) h p ==>
+              (hist_bind (to_hist (fun h_ -> io_pre h_ o args) (fun h_ res_ lt_ -> io_post h_ o args res_ /\ lt_ == [op_to_ev o args res_])) (fun (r:io_res o args) -> theta (Return r))) h p) by (compute ());
+      eliminate forall (lt':local_trace h) (r':io_res o args). lt' == [op_to_ev o args r'] ==>
+        (theta (Return r')) (h++lt') (fun (lt'':local_trace (h++lt')) (r'':io_res o args) -> p (lt' @ lt'') r'')
+        with [op_to_ev o args res] res
     end
   end
-
-#push-options "--split_queries always"
-let rec theta_thetaP_in_post #t (m:io t) (h:history) : Lemma (theta m h (fun lt fs_r -> thetaP m h lt fs_r)) =
-  match m with
-  | Return x -> ()
-  | Call o args k ->
-      introduce forall (lt:local_trace h) (r:io_res o args). (lt == [op_to_ev o args r]) ==> theta (k r) (h ++ lt) (fun lt' fs_r' -> thetaP m h (lt@lt') fs_r') with begin
-        introduce _ ==> _ with _. begin
-          theta_thetaP_in_post (k r) (h ++ lt);
-          assert (theta (k r) (h ++ lt) (fun lt' fs_r' -> thetaP (k r) (h ++ lt) lt' fs_r'));
-          thetaP_shift_op_lt o args k r h lt;
-          assert (theta (k r) (h ++ lt) (fun lt' fs_r' -> thetaP m h (lt@lt') fs_r'))
-        end
-      end;
-      assert ((op_wp o args) h (fun lt fs_r -> theta (k fs_r) (h ++ lt) (fun lt' fs_r' -> thetaP m h (lt@lt') fs_r')))
 #pop-options
-
-unfold
-let theta_io_bind_exists_post #t1 #t2 (m:io t1) (f:t1 -> io t2) (h:history) (lt:local_trace h) (fs_r:t2) =
-  exists fs_m lt1 lt2 .
-      lt = lt1 @ lt2 /\
-      thetaP m h lt1 fs_m /\
-      thetaP (f fs_m) (h ++ lt1) lt2 fs_r
-
-#push-options "--split_queries always"
-let rec theta_io_bind_exists_ #t1 #t2 (m:io t1) (f:t1 -> io t2) (h:history) : Lemma (theta (io_bind m f) h (theta_io_bind_exists_post m f h)) =
-  match m with
-  | Return x ->
-      theta_thetaP_in_post (f x) h;
-      assert (theta (f x) h (fun lt fs_r -> thetaP (f x) h lt fs_r));
-      calc (hist_post_ord) {
-        (fun lt fs_r -> thetaP (f x) h lt fs_r);
-        `hist_post_ord` {}
-        (fun lt fs_r -> exists lt2. lt = []@lt2 /\ thetaP (f x) h lt2 fs_r);
-        `hist_post_ord` {}
-        (fun lt fs_r -> exists fs_m lt1 lt2. lt = lt1@lt2 /\ thetaP (Return x) h lt1 fs_m /\ thetaP (f fs_m) (h++lt1) lt2 fs_r);
-      };
-      assert (theta (f x) h (theta_io_bind_exists_post m f h))
-  | Call o args k ->
-      introduce forall lt r. lt == [op_to_ev o args r] ==> theta (io_bind (k r) f) (h ++ lt) (fun lt' fs_r' -> theta_io_bind_exists_post m f h (lt @ lt') fs_r') with begin
-        introduce _ ==> _ with _. begin
-          theta_io_bind_exists_ (k r) f (h ++ lt);
-          introduce forall (lt':local_trace (h ++ lt)) fs_r' . theta_io_bind_exists_post (k r) f (h ++ lt) lt' fs_r' ==> theta_io_bind_exists_post m f h (lt @ lt') fs_r' with begin
-            introduce _ ==> _ with _. begin
-              eliminate exists fs_m lt1 lt2 .
-                            lt' = lt1 @ lt2 /\
-                            thetaP (k r) (h ++ lt) lt1 fs_m /\
-                            thetaP (f fs_m) (h ++ lt ++ lt1) lt2 fs_r'
-              returns theta_io_bind_exists_post m f h (lt @ lt') fs_r'
-              with _. begin
-                trans_history h lt lt1;
-                introduce exists fs_m' lt1' lt2' .
-                              lt @ lt' = lt1' @ lt2' /\
-                              thetaP m h lt1' fs_m /\
-                              thetaP (f fs_m) (h ++ lt1') lt2' fs_r'
-                with fs_m (lt @ lt1) lt2
-                and begin
-                  thetaP_shift_op_lt o args k r h lt
-                end
-              end
-            end
-          end;
-          assert (theta (io_bind (k r) f) (h ++ lt) (fun lt' r' -> theta_io_bind_exists_post m f h (lt @ lt') r'))
-        end
-      end;
-      assert (hist_bind (op_wp o args) (fun r -> theta (io_bind (k r) f)) h (theta_io_bind_exists_post m f h));
-      assert (theta (io_bind (Call o args k) f) h (theta_io_bind_exists_post m f h))
-#pop-options
-
-let theta_io_bind_exists #t1 #t2 (m:io t1) (f:t1 -> io t2) (h:history) : Lemma (theta (io_bind m f) h (theta_io_bind_exists_post m f h)) =
-  theta_io_bind_exists_ m f h
-
-val destruct_fs_beh #t1 #t2 (m:io t1) (k:t1 -> io t2) (h:history) (lt:local_trace h) (fs_r:t2) :
-  Lemma
-    (requires thetaP (io_bind m k) h lt fs_r)
-    (ensures exists (lt1:local_trace h) (lt2:local_trace (h++lt1)) (fs_m:t1).
-      lt == (lt1@lt2) /\
-      thetaP m h lt1 fs_m /\
-      thetaP (k fs_m) (h++lt1) lt2 fs_r)
-let destruct_fs_beh #t1 #t2 (m:io t1) (k:t1 -> io t2) (h:history) (lt:local_trace h) (fs_r:t2) :
-  Lemma
-    (requires thetaP (io_bind m k) h lt fs_r) // forall p. theta (io_bind m k) h p ==> p lt fs_r
-    (ensures exists (lt1:local_trace h) (lt2:local_trace (h++lt1)) (fs_m:t1).
-      lt == (lt1@lt2) /\
-      thetaP m h lt1 fs_m /\ // forall p. theta m h p ==> p lt1 fs_m
-      thetaP (k fs_m) (h++lt1) lt2 fs_r) (* forall p. theta (k fs_m) (h++lt1) p ==> p lt2 fs_r *) =
-    theta_io_bind_exists m k h
